SeparationLogic/MainSoundnessResult.v
@@ -1,0 +1,136 @@
+Require Import Coq.Logic.Classical_Prop.
+Require Import Logic.lib.Coqlib.
+Require Import Logic.LogicBase.
+Require Import Logic.MinimunLogic.MinimunLogic.
+Require Import Logic.PropositionalLogic.Syntax.
+Require Import Logic.SeparationLogic.Syntax.
+Require Import Logic.PropositionalLogic.KripkeSemantics.
+Require Import Logic.SeparationLogic.QinxiangSantiagoSemantics.
+Require Import Logic.PropositionalLogic.IntuitionisticPropositionalLogic.
+Require Import Logic.SeparationLogic.SeparationLogic.
+
+Local Open Scope logic_base.
+Local Open Scope PropositionalLogic.
+Local Open Scope SeparationLogic.
+
+Lemma sound_sepcon_comm {L: Language} {nL: NormalLanguage L} {pL: PropositionalLanguage L} {SL: SeparationLanguage L} {SM: Semantics L} {pkS: PreKripkeSemantics L SM} {kiSM: KripkeIntuitionisticSemantics L SM} {qsSM: QinxiangSantiagoSemantics L SM}:
+  forall x y: expr,
+    forall M m,
+      KRIPKE: M, m |= x * y --> y * x.
+Proof.
+  intros.
+  rewrite sat_impp; intros.
+  rewrite sat_sepcon in H0 |- *; intros.
+  destruct H0 as [m1 [m2 [? [? ?]]]].
+  exists m2, m1.
+  split; [| split]; auto.
+  apply join_comm; auto.
+Qed.
+
+Lemma sound_sepcon_assoc {L: Language} {nL: NormalLanguage L} {pL: PropositionalLanguage L} {SL: SeparationLanguage L} {SM: Semantics L} {pkS: PreKripkeSemantics L SM} {kiSM: KripkeIntuitionisticSemantics L SM} {qsSM: QinxiangSantiagoSemantics L SM}:
+  forall x y z: expr,
+    forall M m,
+      KRIPKE: M, m |= x * (y * z) <--> (x * y) * z.
+Proof.
+  intros.
+  unfold iffp.
+  rewrite sat_andp.
+  split; intros.
+  + rewrite sat_impp; intros.
+    rewrite sat_sepcon in H0.
+    destruct H0 as [mx [myz [? [? ?]]]].
+    rewrite sat_sepcon in H2.
+    destruct H2 as [my [mz [? [? ?]]]].
+    apply join_comm in H0.
+    apply join_comm in H2.
+    destruct (join_assoc _ mz my mx myz n H2 H0) as [mxy [? ?]].
+    apply join_comm in H5.
+    apply join_comm in H6.
+    rewrite sat_sepcon.
+    exists mxy, mz.
+    split; [| split]; auto.
+    rewrite sat_sepcon.
+    exists mx, my.
+    split; [| split]; auto.
+  + rewrite sat_impp; intros.
+    rewrite sat_sepcon in H0.
+    destruct H0 as [mxy [mz [? [? ?]]]].
+    rewrite sat_sepcon in H1.
+    destruct H1 as [mx [my [? [? ?]]]].
+    destruct (join_assoc _ mx my mz mxy n H1 H0) as [myz [? ?]].
+    rewrite sat_sepcon.
+    exists mx, myz.
+    split; [| split]; auto.
+    rewrite sat_sepcon.
+    exists my, mz.
+    split; [| split]; auto.
+Qed.
+
+Lemma sound_wand_sepcon_adjoint {L: Language} {nL: NormalLanguage L} {pL: PropositionalLanguage L} {SL: SeparationLanguage L} {SM: Semantics L} {pkS: PreKripkeSemantics L SM} {kiSM: KripkeIntuitionisticSemantics L SM} {qsSM: QinxiangSantiagoSemantics L SM}:
+  forall x y z: expr,
+    forall M,
+     (forall m, KRIPKE: M, m |= x * y --> z) <-> (forall m, KRIPKE: M, m |= x --> (y -* z)).
+Proof.
+  intros.
+  pose proof Korder_PreOrder M as H_PreOrder.
+  split; intro.
+  + assert (ASSU: forall m1 m2 m, join m1 m2 m -> KRIPKE: M, m1 |= x -> KRIPKE: M, m2 |= y -> KRIPKE: M, m |= z).
+    Focus 1. {
+      intros.
+      specialize (H m).
+      rewrite sat_impp in H.
+      apply (H m); [reflexivity |].
+      rewrite sat_sepcon.
+      exists m1, m2; auto.
+    } Unfocus.
+    clear H.
+    intros.
+    rewrite sat_impp; intros.
+    rewrite sat_wand; intros.
+    apply (ASSU m0 m1 m2); auto.
+    eapply sat_mono; eauto.
+  + assert (ASSU: forall m0 m1 m2 m, Korder m0 m -> join m0 m1 m2 -> KRIPKE: M, m |= x -> KRIPKE: M, m1 |= y -> KRIPKE: M, m2 |= z).
+    Focus 1. {
+      intros.
+      specialize (H m).
+      rewrite sat_impp in H.
+      revert m0 m1 m2 H0 H1 H3.
+      rewrite <- sat_wand.
+      apply (H m); [reflexivity | auto].
+    } Unfocus.
+    intros.
+    rewrite sat_impp; intros.
+    rewrite sat_sepcon in H1.
+    destruct H1 as [m1 [m2 [? [? ?]]]].
+    apply (ASSU m1 m2 n m1); auto.
+    reflexivity.
+Qed.
+
+Lemma sound_sepcon_mono {L: Language} {nL: NormalLanguage L} {pL: PropositionalLanguage L} {SL: SeparationLanguage L} {SM: Semantics L} {pkS: PreKripkeSemantics L SM} {kiSM: KripkeIntuitionisticSemantics L SM} {qsSM: QinxiangSantiagoSemantics L SM}:
+  forall x1 x2 y1 y2: expr,
+    forall M,
+     (forall m, KRIPKE: M, m |= x1 --> x2) ->
+     (forall m, KRIPKE: M, m |= y1 --> y2) ->
+     (forall m, KRIPKE: M, m |= x1 * y1 --> x2 * y2).
+Proof.
+  intros.
+  pose proof Korder_PreOrder M as H_PreOrder.
+  assert (ASSUx: forall m, KRIPKE: M, m |= x1 -> KRIPKE: M, m |= x2).
+  Focus 1. {
+    intros.
+    specialize (H m0).
+    rewrite sat_impp in H.
+    apply (H m0); [reflexivity | auto].
+  } Unfocus.
+  assert (ASSUy: forall m, KRIPKE: M, m |= y1 -> KRIPKE: M, m |= y2).
+  Focus 1. {
+    intros.
+    specialize (H0 m0).
+    rewrite sat_impp in H0.
+    apply (H0 m0); [reflexivity | auto].
+  } Unfocus.
+  rewrite sat_impp; intros.
+  rewrite sat_sepcon in H2 |- *.
+  destruct H2 as [m1 [m2 [? [? ?]]]].
+  exists m1, m2; auto.
+Qed.
