SeparationLogic/MainSoundnessResult_Fail.v
@@ -1,0 +1,44 @@
+Require Import Coq.Logic.Classical_Prop.
+Require Import Logic.lib.Coqlib.
+Require Import Logic.LogicBase.
+Require Import Logic.MinimunLogic.MinimunLogic.
+Require Import Logic.PropositionalLogic.Syntax.
+Require Import Logic.SeparationLogic.Syntax.
+Require Import Logic.PropositionalLogic.KripkeSemantics.
+Require Import Logic.SeparationLogic.QinxiangSantiagoSemantics_Fail.
+Require Import Logic.PropositionalLogic.IntuitionisticPropositionalLogic.
+Require Import Logic.SeparationLogic.SeparationLogic.
+
+Local Open Scope logic_base.
+Local Open Scope PropositionalLogic.
+Local Open Scope SeparationLogic.
+
+Lemma sound_sepcon_comm {L: Language} {nL: NormalLanguage L} {pL: PropositionalLanguage L} {SL: SeparationLanguage L} {SM: Semantics L} {pkS: PreKripkeSemantics L SM} {kiSM: KripkeIntuitionisticSemantics L SM} {qsSM: QinxiangSantiagoSemantics L SM}:
+  forall x y: expr,
+    forall M m,
+      KRIPKE: M, m |= x * y --> y * x.
+Proof.
+  intros.
+  pose proof Korder_PreOrder M as H_PreOrder.
+  rewrite sat_impp; intros.
+  rewrite sat_sepcon in H0 |- *; intros.
+  destruct H0 as [m0 [m1 [m2 [? [? [? ?]]]]]].
+  exists m0, m2, m1.
+  split; [| split; [| split]]; auto.
+  apply join_comm; auto.
+Qed.
+
+Lemma sound_sepcon_assoc {L: Language} {nL: NormalLanguage L} {pL: PropositionalLanguage L} {SL: SeparationLanguage L} {SM: Semantics L} {pkS: PreKripkeSemantics L SM} {kiSM: KripkeIntuitionisticSemantics L SM} {qsSM: QinxiangSantiagoSemantics L SM}:
+  forall x y z: expr,
+    forall M m,
+      KRIPKE: M, m |= x * (y * z) <--> (x * y) * z.
+Proof.
+  intros.
+  unfold iffp.
+  rewrite sat_andp.
+  split; intros.
+  + rewrite sat_impp; intros.
+    rewrite sat_sepcon in H0.
+    destruct H0 as [m0 [m1 [m2 [? [? [? ?]]]]]].
+    (* fail *)
+Abort.
