SeparationLogic/QinxiangSantiagoSemantics_Fail.v
@@ -1,0 +1,27 @@
+Require Import Coq.Logic.Classical_Prop.
+Require Import Logic.lib.Coqlib.
+Require Import Logic.LogicBase.
+Require Import Logic.MinimunLogic.MinimunLogic.
+Require Import Logic.PropositionalLogic.Syntax.
+Require Import Logic.SeparationLogic.Syntax.
+Require Import Logic.PropositionalLogic.KripkeSemantics.
+
+Local Open Scope logic_base.
+Local Open Scope PropositionalLogic.
+Local Open Scope SeparationLogic.
+
+Class QinxiangSantiagoSemantics (L: Language) {nL: NormalLanguage L} {pL: PropositionalLanguage L} {SL: SeparationLanguage L} (SM: Semantics L) {pkSM: PreKripkeSemantics L SM} {kiSM: KripkeIntuitionisticSemantics L SM} : Type := {
+  join: forall {M: Kmodel}, Kworlds M -> Kworlds M -> Kworlds M -> Prop;
+  join_comm: forall M (m1 m2 m: Kworlds M), join m1 m2 m -> join m2 m1 m;
+  join_assoc: forall M (mx my mz mxy mxyz: Kworlds M), join mx my mxy -> join mxy mz mxyz -> exists myz, join my mz myz /\ join mx myz mxyz;
+  sat_sepcon: forall M m x y, KRIPKE: M , m |= x * y <-> exists m0 m1 m2, Korder m m0 /\ join m1 m2 m0 /\ KRIPKE: M , m1 |= x /\ KRIPKE: M, m2 |= y;
+  sat_wand: forall M m x y, KRIPKE: M , m |= x -* y <-> forall m0 m1 m2, Korder m0 m -> join m1 m0 m2 -> KRIPKE: M , m1 |= x -> KRIPKE: M, m2 |= y
+}.
+
+(*
+
+  sat_sepcon: forall M m x y, KRIPKE: M , m |= x * y <-> exists m1 m2, join m1 m2 m /\ KRIPKE: M , m1 |= x /\ KRIPKE: M, m2 |= y;
+  sat_wand: forall M m x y, KRIPKE: M , m |= x -* y <-> forall m1 m2, join m1 m m2 -> KRIPKE: M , m1 |= x -> KRIPKE: M, m2 |= y
+
+*)
+
