SeparationLogic/SeparationLogic.v
@@ -1,0 +1,85 @@
+Require Import Coq.Logic.Classical_Prop.
+Require Import Logic.lib.Coqlib.
+Require Import Logic.LogicBase.
+Require Import Logic.MinimunLogic.MinimunLogic.
+Require Import Logic.MinimunLogic.ContextProperty.
+Require Import Logic.PropositionalLogic.Syntax.
+Require Import Logic.PropositionalLogic.IntuitionisticPropositionalLogic.
+Require Import Logic.SeparationLogic.Syntax.
+
+Local Open Scope logic_base.
+Local Open Scope PropositionalLogic.
+Local Open Scope SeparationLogic.
+
+Class SeparationLogic (L: Language) {nL: NormalLanguage L} {pL: PropositionalLanguage L} {SL: SeparationLanguage L} (Gamma: ProofTheory L) {mpGamma: MinimunPropositionalLogic L Gamma} {ipGamma: IntuitionisticPropositionalLogic L Gamma} := {
+  sepcon_comm: forall x y, |-- x * y --> y * x;
+  sepcon_assoc: forall x y z, |-- x * (y * z) <--> (x * y) * z;
+  wand_sepcon_adjoin: forall x y z, |-- x * y --> z <-> |-- x --> (y -* z);
+  sepcon_mono: forall x1 x2 y1 y2, |-- x1 --> x2 -> |-- y1 --> y2 -> |-- (x1 * y1) --> (x2 * y2)
+}.
+
+Module SeparationLogic.
+Section SeparationLogic.
+
+Context (Var: Type).
+
+Instance L: Language := SeparationLanguage.L Var.
+Instance nL: NormalLanguage L := SeparationLanguage.nL Var.
+Instance pL: PropositionalLanguage L := SeparationLanguage.pL Var.
+Instance SL: SeparationLanguage L := SeparationLanguage.SL Var.
+
+Inductive provable: expr -> Prop :=
+| modus_ponens: forall x y, provable (x --> y) -> provable x -> provable y
+| axiom1: forall x y, provable (x --> (y --> x))
+| axiom2: forall x y z, provable ((x --> y --> z) --> (x --> y) --> (x --> z))
+| andp_intros: forall x y, provable (x --> y --> x && y)
+| andp_elim1: forall x y, provable (x && y --> x)
+| andp_elim2: forall x y, provable (x && y --> y)
+| orp_intros1: forall x y, provable (x --> x || y)
+| orp_intros2: forall x y, provable (y --> x || y)
+| orp_elim: forall x y z, provable ((x --> z) --> (y --> z) --> (x || y --> z))
+| falsep_elim: forall x, provable (FF --> x)
+| sepcon_comm: forall x y, provable (x * y --> y * x)
+| sepcon_assoc: forall x y z, provable (x * (y * z) <--> (x * y) * z)
+| wand_sepcon_adjoint1: forall x y z, provable (x * y --> z) -> provable (x --> (y -* z))
+| wand_sepcon_adjoint2: forall x y z, provable (x --> (y -* z)) -> provable (x * y --> z)
+| sepcon_mono: forall x1 x2 y1 y2, provable (x1 --> x2) -> provable (y1 --> y2) -> provable ((x1 * y1) --> (x2 * y2)).
+
+Instance G: ProofTheory L := Build_AxiomaticProofTheory provable.
+
+Instance nG: NormalProofTheory L G := Build_nAxiomaticProofTheory provable.
+
+Instance mpG: MinimunPropositionalLogic L G.
+Proof.
+  constructor.
+  + apply modus_ponens.
+  + apply axiom1.
+  + apply axiom2.
+Qed.
+
+Instance ipG: IntuitionisticPropositionalLogic L G.
+Proof.
+  constructor.
+  + apply andp_intros.
+  + apply andp_elim1.
+  + apply andp_elim2.
+  + apply orp_intros1.
+  + apply orp_intros2.
+  + apply orp_elim.
+  + apply falsep_elim.
+Qed.
+
+Instance sG: SeparationLogic L G.
+Proof.
+  constructor.
+  + apply sepcon_comm.
+  + apply sepcon_assoc.
+  + intros; split.
+    - apply wand_sepcon_adjoint1.
+    - apply wand_sepcon_adjoint2.
+  + apply sepcon_mono.
+Qed.
+
+End SeparationLogic.
+End SeparationLogic.
+
