Makefile
@@ -9,8 +9,10 @@ all: Wf.vo base.vo IPC.vo trivial.vo Kripke.vo enumerate.vo LogicBase.vo \
      PropositionalLogic/IntuitionisticPropositionalLogic.vo \
      PropositionalLogic/KripkeSemantics.vo \
      PropositionalLogic/Syntax.vo PropositionalLogic/ClassicalPropositionalLogic.vo \
-     PropositionalLogic/WeakClassicalPropositionalLogic.vo \
+     PropositionalLogic/GodelDummettLogic.vo \
      PropositionalLogic/TrivialSemantics.vo PropositionalLogic/Sound_Classical_Trivial.vo \
      PropositionalLogic/Complete_Classical_Trivial.vo lib/Coqlib.vo \
      lib/Bijection.vo lib/Countable.vo PropositionalLogic/Complete_Intuitionistic_Kripke.vo \
-     PropositionalLogic/Complete_Kripke.vo PropositionalLogic/Sound_Kripke.vo
+     PropositionalLogic/Complete_Kripke.vo PropositionalLogic/Sound_Kripke.vo \
+     SeparationLogic/Syntax.vo SeparationLogic/SeparationLogic.vo \
+     SeparationLogic/QinxiangSantiagoSemantics.vo
